src/HOL/IMP/Compiler0.thy
@@ -1,0 +1,272 @@
+(*  Title:      HOL/IMP/Compiler.thy
+    ID:         $Id$
+    Author:     Tobias Nipkow, TUM
+    Copyright   1996 TUM
+
+This is an early version of the compiler, where the abstract machine
+has an explicit pc. This turned out to be awkward, and a second
+development was started. See Machines.thy and Compiler.thy.
+*)
+
+header "A Simple Compiler"
+
+theory Compiler0 = Natural:
+
+subsection "An abstract, simplistic machine"
+
+text {* There are only three instructions: *}
+datatype instr = ASIN loc aexp | JMPF bexp nat | JMPB nat
+
+text {* We describe execution of programs in the machine by
+  an operational (small step) semantics:
+*}
+consts  stepa1 :: "instr list \<Rightarrow> ((state\<times>nat) \<times> (state\<times>nat))set"
+
+syntax
+  "_stepa1" :: "[instr list,state,nat,state,nat] \<Rightarrow> bool"
+               ("_ |- (3<_,_>/ -1-> <_,_>)" [50,0,0,0,0] 50)
+  "_stepa" :: "[instr list,state,nat,state,nat] \<Rightarrow> bool"
+               ("_ |-/ (3<_,_>/ -*-> <_,_>)" [50,0,0,0,0] 50)
+
+  "_stepan" :: "[instr list,state,nat,nat,state,nat] \<Rightarrow> bool"
+               ("_ |-/ (3<_,_>/ -(_)-> <_,_>)" [50,0,0,0,0,0] 50)
+
+syntax (xsymbols)
+  "_stepa1" :: "[instr list,state,nat,state,nat] \<Rightarrow> bool"
+               ("_ \<turnstile> (3\<langle>_,_\<rangle>/ -1\<rightarrow> \<langle>_,_\<rangle>)" [50,0,0,0,0] 50)
+  "_stepa" :: "[instr list,state,nat,state,nat] \<Rightarrow> bool"
+               ("_ \<turnstile>/ (3\<langle>_,_\<rangle>/ -*\<rightarrow> \<langle>_,_\<rangle>)" [50,0,0,0,0] 50)
+  "_stepan" :: "[instr list,state,nat,nat,state,nat] \<Rightarrow> bool"
+               ("_ \<turnstile>/ (3\<langle>_,_\<rangle>/ -(_)\<rightarrow> \<langle>_,_\<rangle>)" [50,0,0,0,0,0] 50)
+
+translations  
+  "P \<turnstile> \<langle>s,m\<rangle> -1\<rightarrow> \<langle>t,n\<rangle>" == "((s,m),t,n) : stepa1 P"
+  "P \<turnstile> \<langle>s,m\<rangle> -*\<rightarrow> \<langle>t,n\<rangle>" == "((s,m),t,n) : ((stepa1 P)^*)"
+  "P \<turnstile> \<langle>s,m\<rangle> -(i)\<rightarrow> \<langle>t,n\<rangle>" == "((s,m),t,n) : ((stepa1 P)^i)"
+
+inductive "stepa1 P"
+intros
+ASIN[simp]:
+  "\<lbrakk> n<size P; P!n = ASIN x a \<rbrakk> \<Longrightarrow> P \<turnstile> \<langle>s,n\<rangle> -1\<rightarrow> \<langle>s[x\<mapsto> a s],Suc n\<rangle>"
+JMPFT[simp,intro]:
+  "\<lbrakk> n<size P; P!n = JMPF b i;  b s \<rbrakk> \<Longrightarrow> P \<turnstile> \<langle>s,n\<rangle> -1\<rightarrow> \<langle>s,Suc n\<rangle>"
+JMPFF[simp,intro]:
+  "\<lbrakk> n<size P; P!n = JMPF b i; ~b s; m=n+i \<rbrakk> \<Longrightarrow> P \<turnstile> \<langle>s,n\<rangle> -1\<rightarrow> \<langle>s,m\<rangle>"
+JMPB[simp]:
+  "\<lbrakk> n<size P; P!n = JMPB i; i <= n; j = n-i \<rbrakk> \<Longrightarrow> P \<turnstile> \<langle>s,n\<rangle> -1\<rightarrow> \<langle>s,j\<rangle>"
+
+subsection "The compiler"
+
+consts compile :: "com \<Rightarrow> instr list"
+primrec
+"compile \<SKIP> = []"
+"compile (x:==a) = [ASIN x a]"
+"compile (c1;c2) = compile c1 @ compile c2"
+"compile (\<IF> b \<THEN> c1 \<ELSE> c2) =
+ [JMPF b (length(compile c1) + 2)] @ compile c1 @
+ [JMPF (%x. False) (length(compile c2)+1)] @ compile c2"
+"compile (\<WHILE> b \<DO> c) = [JMPF b (length(compile c) + 2)] @ compile c @
+ [JMPB (length(compile c)+1)]"
+
+declare nth_append[simp]
+
+subsection "Context lifting lemmas"
+
+text {* 
+  Some lemmas for lifting an execution into a prefix and suffix
+  of instructions; only needed for the first proof.
+*}
+lemma app_right_1:
+  assumes A: "is1 \<turnstile> \<langle>s1,i1\<rangle> -1\<rightarrow> \<langle>s2,i2\<rangle>"
+  shows "is1 @ is2 \<turnstile> \<langle>s1,i1\<rangle> -1\<rightarrow> \<langle>s2,i2\<rangle>"
+proof -
+ from A show ?thesis
+ by induct force+
+qed
+
+lemma app_left_1:
+  assumes A: "is2 \<turnstile> \<langle>s1,i1\<rangle> -1\<rightarrow> \<langle>s2,i2\<rangle>"
+  shows "is1 @ is2 \<turnstile> \<langle>s1,size is1+i1\<rangle> -1\<rightarrow> \<langle>s2,size is1+i2\<rangle>"
+proof -
+ from A show ?thesis
+ by induct force+
+qed
+
+declare rtrancl_induct2 [induct set: rtrancl]
+
+lemma app_right:
+assumes A: "is1 \<turnstile> \<langle>s1,i1\<rangle> -*\<rightarrow> \<langle>s2,i2\<rangle>"
+shows "is1 @ is2 \<turnstile> \<langle>s1,i1\<rangle> -*\<rightarrow> \<langle>s2,i2\<rangle>"
+proof -
+ from A show ?thesis
+ proof induct
+   show "is1 @ is2 \<turnstile> \<langle>s1,i1\<rangle> -*\<rightarrow> \<langle>s1,i1\<rangle>" by simp
+ next
+   fix s1' i1' s2 i2
+   assume "is1 @ is2 \<turnstile> \<langle>s1,i1\<rangle> -*\<rightarrow> \<langle>s1',i1'\<rangle>"
+          "is1 \<turnstile> \<langle>s1',i1'\<rangle> -1\<rightarrow> \<langle>s2,i2\<rangle>"
+   thus "is1 @ is2 \<turnstile> \<langle>s1,i1\<rangle> -*\<rightarrow> \<langle>s2,i2\<rangle>"
+     by(blast intro:app_right_1 rtrancl_trans)
+ qed
+qed
+
+lemma app_left:
+assumes A: "is2 \<turnstile> \<langle>s1,i1\<rangle> -*\<rightarrow> \<langle>s2,i2\<rangle>"
+shows "is1 @ is2 \<turnstile> \<langle>s1,size is1+i1\<rangle> -*\<rightarrow> \<langle>s2,size is1+i2\<rangle>"
+proof -
+  from A show ?thesis
+  proof induct
+    show "is1 @ is2 \<turnstile> \<langle>s1,length is1 + i1\<rangle> -*\<rightarrow> \<langle>s1,length is1 + i1\<rangle>" by simp
+  next
+    fix s1' i1' s2 i2
+    assume "is1 @ is2 \<turnstile> \<langle>s1,length is1 + i1\<rangle> -*\<rightarrow> \<langle>s1',length is1 + i1'\<rangle>"
+           "is2 \<turnstile> \<langle>s1',i1'\<rangle> -1\<rightarrow> \<langle>s2,i2\<rangle>"
+    thus "is1 @ is2 \<turnstile> \<langle>s1,length is1 + i1\<rangle> -*\<rightarrow> \<langle>s2,length is1 + i2\<rangle>"
+      by(blast intro:app_left_1 rtrancl_trans)
+ qed
+qed
+
+lemma app_left2:
+  "\<lbrakk> is2 \<turnstile> \<langle>s1,i1\<rangle> -*\<rightarrow> \<langle>s2,i2\<rangle>; j1 = size is1+i1; j2 = size is1+i2 \<rbrakk> \<Longrightarrow>
+   is1 @ is2 \<turnstile> \<langle>s1,j1\<rangle> -*\<rightarrow> \<langle>s2,j2\<rangle>"
+  by (simp add:app_left)
+
+lemma app1_left:
+  "is \<turnstile> \<langle>s1,i1\<rangle> -*\<rightarrow> \<langle>s2,i2\<rangle> \<Longrightarrow>
+   instr # is \<turnstile> \<langle>s1,Suc i1\<rangle> -*\<rightarrow> \<langle>s2,Suc i2\<rangle>"
+  by(erule app_left[of _ _ _ _ _ "[instr]",simplified])
+
+subsection "Compiler correctness"
+
+declare rtrancl_into_rtrancl[trans]
+        converse_rtrancl_into_rtrancl[trans]
+        rtrancl_trans[trans]
+
+text {*
+  The first proof; The statement is very intuitive,
+  but application of induction hypothesis requires the above lifting lemmas
+*}
+theorem assumes A: "\<langle>c,s\<rangle> \<longrightarrow>\<^sub>c t"
+shows "compile c \<turnstile> \<langle>s,0\<rangle> -*\<rightarrow> \<langle>t,length(compile c)\<rangle>" (is "?P c s t")
+proof -
+  from A show ?thesis
+  proof induct
+    show "\<And>s. ?P \<SKIP> s s" by simp
+  next
+    show "\<And>a s x. ?P (x :== a) s (s[x\<mapsto> a s])" by force
+  next
+    fix c0 c1 s0 s1 s2
+    assume "?P c0 s0 s1"
+    hence "compile c0 @ compile c1 \<turnstile> \<langle>s0,0\<rangle> -*\<rightarrow> \<langle>s1,length(compile c0)\<rangle>"
+      by(rule app_right)
+    moreover assume "?P c1 s1 s2"
+    hence "compile c0 @ compile c1 \<turnstile> \<langle>s1,length(compile c0)\<rangle> -*\<rightarrow>
+           \<langle>s2,length(compile c0)+length(compile c1)\<rangle>"
+    proof -
+      show "\<And>is1 is2 s1 s2 i2.
+	      is2 \<turnstile> \<langle>s1,0\<rangle> -*\<rightarrow> \<langle>s2,i2\<rangle> \<Longrightarrow>
+	      is1 @ is2 \<turnstile> \<langle>s1,size is1\<rangle> -*\<rightarrow> \<langle>s2,size is1+i2\<rangle>"
+	using app_left[of _ 0] by simp
+    qed
+    ultimately have "compile c0 @ compile c1 \<turnstile> \<langle>s0,0\<rangle> -*\<rightarrow>
+                       \<langle>s2,length(compile c0)+length(compile c1)\<rangle>"
+      by (rule rtrancl_trans)
+    thus "?P (c0; c1) s0 s2" by simp
+  next
+    fix b c0 c1 s0 s1
+    let ?comp = "compile(\<IF> b \<THEN> c0 \<ELSE> c1)"
+    assume "b s0" and IH: "?P c0 s0 s1"
+    hence "?comp \<turnstile> \<langle>s0,0\<rangle> -1\<rightarrow> \<langle>s0,1\<rangle>" by auto
+    also from IH
+    have "?comp \<turnstile> \<langle>s0,1\<rangle> -*\<rightarrow> \<langle>s1,length(compile c0)+1\<rangle>"
+      by(auto intro:app1_left app_right)
+    also have "?comp \<turnstile> \<langle>s1,length(compile c0)+1\<rangle> -1\<rightarrow> \<langle>s1,length ?comp\<rangle>"
+      by(auto)
+    finally show "?P (\<IF> b \<THEN> c0 \<ELSE> c1) s0 s1" .
+  next
+    fix b c0 c1 s0 s1
+    let ?comp = "compile(\<IF> b \<THEN> c0 \<ELSE> c1)"
+    assume "\<not>b s0" and IH: "?P c1 s0 s1"
+    hence "?comp \<turnstile> \<langle>s0,0\<rangle> -1\<rightarrow> \<langle>s0,length(compile c0) + 2\<rangle>" by auto
+    also from IH
+    have "?comp \<turnstile> \<langle>s0,length(compile c0)+2\<rangle> -*\<rightarrow> \<langle>s1,length ?comp\<rangle>"
+      by(force intro!:app_left2 app1_left)
+    finally show "?P (\<IF> b \<THEN> c0 \<ELSE> c1) s0 s1" .
+  next
+    fix b c and s::state
+    assume "\<not>b s"
+    thus "?P (\<WHILE> b \<DO> c) s s" by force
+  next
+    fix b c and s0::state and s1 s2
+    let ?comp = "compile(\<WHILE> b \<DO> c)"
+    assume "b s0" and
+      IHc: "?P c s0 s1" and IHw: "?P (\<WHILE> b \<DO> c) s1 s2"
+    hence "?comp \<turnstile> \<langle>s0,0\<rangle> -1\<rightarrow> \<langle>s0,1\<rangle>" by auto
+    also from IHc
+    have "?comp \<turnstile> \<langle>s0,1\<rangle> -*\<rightarrow> \<langle>s1,length(compile c)+1\<rangle>"
+      by(auto intro:app1_left app_right)
+    also have "?comp \<turnstile> \<langle>s1,length(compile c)+1\<rangle> -1\<rightarrow> \<langle>s1,0\<rangle>" by simp
+    also note IHw
+    finally show "?P (\<WHILE> b \<DO> c) s0 s2".
+  qed
+qed
+
+text {*
+  Second proof; statement is generalized to cater for prefixes and suffixes;
+  needs none of the lifting lemmas, but instantiations of pre/suffix.
+  *}
+theorem "\<langle>c,s\<rangle> \<longrightarrow>\<^sub>c t \<Longrightarrow> 
+  !a z. a@compile c@z \<turnstile> \<langle>s,length a\<rangle> -*\<rightarrow> \<langle>t,length a + length(compile c)\<rangle>";
+apply(erule evalc.induct)
+      apply simp
+     apply(force intro!: ASIN)
+    apply(intro strip)
+    apply(erule_tac x = a in allE)
+    apply(erule_tac x = "a@compile c0" in allE)
+    apply(erule_tac x = "compile c1@z" in allE)
+    apply(erule_tac x = z in allE)
+    apply(simp add:add_assoc[THEN sym])
+    apply(blast intro:rtrancl_trans)
+(* \<IF> b \<THEN> c0 \<ELSE> c1; case b is true *)
+   apply(intro strip)
+   (* instantiate assumption sufficiently for later: *)
+   apply(erule_tac x = "a@[?I]" in allE)
+   apply(simp)
+   (* execute JMPF: *)
+   apply(rule converse_rtrancl_into_rtrancl)
+    apply(force intro!: JMPFT)
+   (* execute compile c0: *)
+   apply(rule rtrancl_trans)
+    apply(erule allE)
+    apply assumption
+   (* execute JMPF: *)
+   apply(rule r_into_rtrancl)
+   apply(force intro!: JMPFF)
+(* end of case b is true *)
+  apply(intro strip)
+  apply(erule_tac x = "a@[?I]@compile c0@[?J]" in allE)
+  apply(simp add:add_assoc)
+  apply(rule converse_rtrancl_into_rtrancl)
+   apply(force intro!: JMPFF)
+  apply(blast)
+ apply(force intro: JMPFF)
+apply(intro strip)
+apply(erule_tac x = "a@[?I]" in allE)
+apply(erule_tac x = a in allE)
+apply(simp)
+apply(rule converse_rtrancl_into_rtrancl)
+ apply(force intro!: JMPFT)
+apply(rule rtrancl_trans)
+ apply(erule allE)
+ apply assumption
+apply(rule converse_rtrancl_into_rtrancl)
+ apply(force intro!: JMPB)
+apply(simp)
+done
+
+text {* Missing: the other direction! I did much of it, and although
+the main lemma is very similar to the one in the new development, the
+lemmas surrounding it seemed much more complicated. In the end I gave
+up. *}
+
+end
