src/HOL/IMP/Machines.thy
@@ -1,0 +1,242 @@
+theory Machines = Natural:
+
+lemma rtrancl_eq: "R^* = Id \<union> (R O R^*)"
+by(fast intro:rtrancl.intros elim:rtranclE)
+
+lemma converse_rtrancl_eq: "R^* = Id \<union> (R^* O R)"
+by(subst r_comp_rtrancl_eq[symmetric], rule rtrancl_eq)
+
+lemmas converse_rel_powE = rel_pow_E2
+
+lemma R_O_Rn_commute: "R O R^n = R^n O R"
+by(induct_tac n, simp, simp add: O_assoc[symmetric])
+
+lemma converse_in_rel_pow_eq:
+"((x,z) \<in> R^n) = (n=0 \<and> z=x \<or> (\<exists>m y. n = Suc m \<and> (x,y) \<in> R \<and> (y,z) \<in> R^m))"
+apply(rule iffI)
+ apply(blast elim:converse_rel_powE)
+apply (fastsimp simp add:gr0_conv_Suc R_O_Rn_commute)
+done
+
+lemma rel_pow_plus: "R^(m+n) = R^n O R^m"
+by(induct n, simp, simp add:O_assoc)
+
+lemma rel_pow_plusI: "\<lbrakk> (x,y) \<in> R^m; (y,z) \<in> R^n \<rbrakk> \<Longrightarrow> (x,z) \<in> R^(m+n)"
+by(simp add:rel_pow_plus rel_compI)
+
+subsection "Instructions"
+
+text {* There are only three instructions: *}
+datatype instr = ASIN loc aexp | JMPF bexp nat | JMPB nat
+
+types instrs = "instr list"
+
+subsection "M0 with PC"
+
+consts  exec01 :: "instr list \<Rightarrow> ((nat\<times>state) \<times> (nat\<times>state))set"
+
+syntax
+  "_exec01" :: "[instrs, nat,state, nat,state] \<Rightarrow> bool"
+               ("(_/ |- (1<_,/_>)/ -1-> (1<_,/_>))" [50,0,0,0,0] 50)
+  "_exec0s" :: "[instrs, nat,state, nat,state] \<Rightarrow> bool"
+               ("(_/ |- (1<_,/_>)/ -*-> (1<_,/_>))" [50,0,0,0,0] 50)
+  "_exec0n" :: "[instrs, nat,state, nat, nat,state] \<Rightarrow> bool"
+               ("(_/ |- (1<_,/_>)/ -_-> (1<_,/_>))" [50,0,0,0,0] 50)
+
+syntax (xsymbols)
+  "_exec01" :: "[instrs, nat,state, nat,state] \<Rightarrow> bool"
+               ("(_/ \<turnstile> (1\<langle>_,/_\<rangle>)/ -1\<rightarrow> (1\<langle>_,/_\<rangle>))" [50,0,0,0,0] 50)
+  "_exec0s" :: "[instrs, nat,state, nat,state] \<Rightarrow> bool"
+               ("(_/ \<turnstile> (1\<langle>_,/_\<rangle>)/ -*\<rightarrow> (1\<langle>_,/_\<rangle>))" [50,0,0,0,0] 50)
+  "_exec0n" :: "[instrs, nat,state, nat, nat,state] \<Rightarrow> bool"
+               ("(_/ \<turnstile> (1\<langle>_,/_\<rangle>)/ -_\<rightarrow> (1\<langle>_,/_\<rangle>))" [50,0,0,0,0] 50)
+
+translations  
+  "p \<turnstile> \<langle>i,s\<rangle> -1\<rightarrow> \<langle>j,t\<rangle>" == "((i,s),j,t) : (exec01 p)"
+  "p \<turnstile> \<langle>i,s\<rangle> -*\<rightarrow> \<langle>j,t\<rangle>" == "((i,s),j,t) : (exec01 p)^*"
+  "p \<turnstile> \<langle>i,s\<rangle> -n\<rightarrow> \<langle>j,t\<rangle>" == "((i,s),j,t) : (exec01 p)^n"
+
+inductive "exec01 P"
+intros
+ASIN: "\<lbrakk> n<size P; P!n = ASIN x a \<rbrakk> \<Longrightarrow> P \<turnstile> \<langle>n,s\<rangle> -1\<rightarrow> \<langle>Suc n,s[x\<mapsto> a s]\<rangle>"
+JMPFT: "\<lbrakk> n<size P; P!n = JMPF b i;  b s \<rbrakk> \<Longrightarrow> P \<turnstile> \<langle>n,s\<rangle> -1\<rightarrow> \<langle>Suc n,s\<rangle>"
+JMPFF: "\<lbrakk> n<size P; P!n = JMPF b i; \<not>b s; m=n+i+1; m \<le> size P \<rbrakk>
+        \<Longrightarrow> P \<turnstile> \<langle>n,s\<rangle> -1\<rightarrow> \<langle>m,s\<rangle>"
+JMPB:  "\<lbrakk> n<size P; P!n = JMPB i; i \<le> n; j = n-i \<rbrakk> \<Longrightarrow> P \<turnstile> \<langle>n,s\<rangle> -1\<rightarrow> \<langle>j,s\<rangle>"
+
+subsection "M0 with lists"
+
+text {* We describe execution of programs in the machine by
+  an operational (small step) semantics:
+*}
+
+types config = "instrs \<times> instrs \<times> state"
+
+consts  stepa1 :: "(config \<times> config)set"
+
+syntax
+  "_stepa1" :: "[instrs,instrs,state, instrs,instrs,state] \<Rightarrow> bool"
+               ("((1<_,/_,/_>)/ -1-> (1<_,/_,/_>))" 50)
+  "_stepa" :: "[instrs,instrs,state, instrs,instrs,state] \<Rightarrow> bool"
+               ("((1<_,/_,/_>)/ -*-> (1<_,/_,/_>))" 50)
+  "_stepan" :: "[state,instrs,instrs, nat, instrs,instrs,state] \<Rightarrow> bool"
+               ("((1<_,/_,/_>)/ -_-> (1<_,/_,/_>))" 50)
+
+syntax (xsymbols)
+  "_stepa1" :: "[instrs,instrs,state, instrs,instrs,state] \<Rightarrow> bool"
+               ("((1\<langle>_,/_,/_\<rangle>)/ -1\<rightarrow> (1\<langle>_,/_,/_\<rangle>))" 50)
+  "_stepa" :: "[instrs,instrs,state, instrs,instrs,state] \<Rightarrow> bool"
+               ("((1\<langle>_,/_,/_\<rangle>)/ -*\<rightarrow> (1\<langle>_,/_,/_\<rangle>))" 50)
+  "_stepan" :: "[instrs,instrs,state, nat, instrs,instrs,state] \<Rightarrow> bool"
+               ("((1\<langle>_,/_,/_\<rangle>)/ -_\<rightarrow> (1\<langle>_,/_,/_\<rangle>))" 50)
+
+translations  
+  "\<langle>p,q,s\<rangle> -1\<rightarrow> \<langle>p',q',t\<rangle>" == "((p,q,s),p',q',t) : stepa1"
+  "\<langle>p,q,s\<rangle> -*\<rightarrow> \<langle>p',q',t\<rangle>" == "((p,q,s),p',q',t) : (stepa1^*)"
+  "\<langle>p,q,s\<rangle> -i\<rightarrow> \<langle>p',q',t\<rangle>" == "((p,q,s),p',q',t) : (stepa1^i)"
+
+
+inductive "stepa1"
+intros
+  "\<langle>ASIN x a#p,q,s\<rangle> -1\<rightarrow> \<langle>p,ASIN x a#q,s[x\<mapsto> a s]\<rangle>"
+  "b s \<Longrightarrow> \<langle>JMPF b i#p,q,s\<rangle> -1\<rightarrow> \<langle>p,JMPF b i#q,s\<rangle>"
+  "\<lbrakk> \<not> b s; i \<le> size p \<rbrakk>
+   \<Longrightarrow> \<langle>JMPF b i # p, q, s\<rangle> -1\<rightarrow> \<langle>drop i p, rev(take i p) @ JMPF b i # q, s\<rangle>"
+  "i \<le> size q
+   \<Longrightarrow> \<langle>JMPB i # p, q, s\<rangle> -1\<rightarrow> \<langle>rev(take i q) @ JMPB i # p, drop i q, s\<rangle>"
+
+inductive_cases execE: "((i#is,p,s),next) : stepa1"
+
+lemma exec_simp[simp]:
+ "(\<langle>i#p,q,s\<rangle> -1\<rightarrow> \<langle>p',q',t\<rangle>) = (case i of
+ ASIN x a \<Rightarrow> t = s[x\<mapsto> a s] \<and> p' = p \<and> q' = i#q |
+ JMPF b n \<Rightarrow> t=s \<and> (if b s then p' = p \<and> q' = i#q
+            else n \<le> size p \<and> p' = drop n p \<and> q' = rev(take n p) @ i # q) |
+ JMPB n \<Rightarrow> n \<le> size q \<and> t=s \<and> p' = rev(take n q) @ i # p \<and> q' = drop n q)"
+apply(rule iffI)
+defer
+apply(clarsimp simp add: stepa1.intros split: instr.split_asm split_if_asm)
+apply(erule execE)
+apply(simp_all)
+done
+
+lemma execn_simp[simp]:
+"(\<langle>i#p,q,s\<rangle> -n\<rightarrow> \<langle>p'',q'',u\<rangle>) =
+ (n=0 \<and> p'' = i#p \<and> q'' = q \<and> u = s \<or>
+  ((\<exists>m p' q' t. n = Suc m \<and>
+                \<langle>i#p,q,s\<rangle> -1\<rightarrow> \<langle>p',q',t\<rangle> \<and> \<langle>p',q',t\<rangle> -m\<rightarrow> \<langle>p'',q'',u\<rangle>)))"
+by(subst converse_in_rel_pow_eq, simp)
+
+
+lemma exec_star_simp[simp]: "(\<langle>i#p,q,s\<rangle> -*\<rightarrow> \<langle>p'',q'',u\<rangle>) =
+ (p'' = i#p & q''=q & u=s |
+ (\<exists>p' q' t. \<langle>i#p,q,s\<rangle> -1\<rightarrow> \<langle>p',q',t\<rangle> \<and> \<langle>p',q',t\<rangle> -*\<rightarrow> \<langle>p'',q'',u\<rangle>))"
+apply(simp add: rtrancl_is_UN_rel_pow del:exec_simp)
+apply(blast)
+done
+
+declare nth_append[simp]
+
+lemma rev_revD: "rev xs = rev ys \<Longrightarrow> xs = ys"
+by simp
+
+lemma [simp]: "(rev xs @ rev ys = rev zs) = (ys @ xs = zs)"
+apply(rule iffI)
+ apply(rule rev_revD, simp)
+apply fastsimp
+done
+
+lemma direction1:
+ "\<langle>q,p,s\<rangle> -1\<rightarrow> \<langle>q',p',t\<rangle> \<Longrightarrow>
+  rev p' @ q' = rev p @ q \<and> rev p @ q \<turnstile> \<langle>size p,s\<rangle> -1\<rightarrow> \<langle>size p',t\<rangle>"
+apply(erule stepa1.induct)
+   apply(simp add:exec01.ASIN)
+  apply(fastsimp intro:exec01.JMPFT)
+ apply simp
+ apply(rule exec01.JMPFF)
+     apply simp
+    apply fastsimp
+   apply simp
+  apply simp
+  apply arith
+ apply simp
+ apply arith
+apply(fastsimp simp add:exec01.JMPB)
+done
+
+lemma drop_take_rev: "\<And>i. drop (length xs - i) (rev xs) = rev (take i xs)"
+apply(induct xs)
+ apply simp_all
+apply(case_tac i)
+apply simp_all
+done
+
+lemma take_drop_rev: "\<And>i. take (length xs - i) (rev xs) = rev (drop i xs)"
+apply(induct xs)
+ apply simp_all
+apply(case_tac i)
+apply simp_all
+done
+
+lemma direction2:
+ "rpq \<turnstile> \<langle>sp,s\<rangle> -1\<rightarrow> \<langle>sp',t\<rangle> \<Longrightarrow>
+ \<forall>p q p' q'. rpq = rev p @ q & sp = size p & sp' = size p' \<longrightarrow>
+          rev p' @ q' = rev p @ q \<longrightarrow> \<langle>q,p,s\<rangle> -1\<rightarrow> \<langle>q',p',t\<rangle>"
+apply(erule exec01.induct)
+   apply(clarsimp simp add: neq_Nil_conv)
+   apply(rule conjI)
+    apply(drule_tac f = "drop (size p')" in arg_cong)
+    apply simp
+    apply(drule sym)
+    apply simp
+   apply(drule_tac f = "take (size p')" in arg_cong)
+   apply simp
+   apply(drule sym)
+   apply simp
+   apply(rule rev_revD)
+   apply simp
+  apply(clarsimp simp add: neq_Nil_conv)
+  apply(rule conjI)
+   apply(drule_tac f = "drop (size p')" in arg_cong)
+   apply simp
+   apply(drule sym)
+   apply simp
+  apply(drule_tac f = "take (size p')" in arg_cong)
+  apply simp
+  apply(drule sym)
+  apply simp
+  apply(rule rev_revD)
+  apply simp
+ apply(clarsimp simp add: neq_Nil_conv)
+ apply(rule conjI)
+  apply(drule_tac f = "drop (size p')" in arg_cong)
+  apply simp
+  apply(drule sym)
+  apply simp
+ apply(drule_tac f = "take (size p')" in arg_cong)
+ apply simp
+ apply(drule sym)
+ apply simp
+ apply(rule rev_revD)
+ apply simp
+apply(clarsimp simp add: neq_Nil_conv)
+apply(rule conjI)
+ apply(drule_tac f = "drop (size p')" in arg_cong)
+ apply simp
+ apply(drule sym)
+ apply(simp add:drop_take_rev)
+apply(drule_tac f = "take (size p')" in arg_cong)
+apply simp
+apply(drule sym)
+apply simp
+apply(rule rev_revD)
+apply(simp add:take_drop_rev)
+done
+
+
+theorem M_eqiv:
+"(\<langle>q,p,s\<rangle> -1\<rightarrow> \<langle>q',p',t\<rangle>) =
+ (rev p' @ q' = rev p @ q \<and> rev p @ q \<turnstile> \<langle>size p,s\<rangle> -1\<rightarrow> \<langle>size p',t\<rangle>)"
+by(fast dest:direction1 direction2)
+
+end
